disk-betree/IndirectionTableModel.i.dfy
@@ -1,22 +1,48 @@
+include "../lib/Maps.s.dfy"
+include "../lib/Option.s.dfy"
+include "../lib/NativeTypes.s.dfy"
+include "../lib/LRU.i.dfy"
+include "../lib/MutableMapModel.i.dfy"
+include "PivotBetreeSpec.i.dfy"
+include "AsyncSectorDiskModel.i.dfy"
+include "BlockCacheSystem.i.dfy"
+
 module IndirectionTableModel {
   import opened Maps
   import opened Options
   import opened NativeTypes
+  import ReferenceType`Internal
   import BT = PivotBetreeSpec`Internal
-  import LBAType
+  import BC = BetreeGraphBlockCache
   import LruModel
+  import MutableMapModel
+
+  datatype Entry = Entry(loc: Option<BC.Location>, succs: seq<BT.G.Reference>)
+  type HashMap = MutableMapModel.LinearHashMap<Entry>
 
   datatype IndirectionTable = IndirectionTable(
-    locs: map<BT.G.Reference, LBAType.Location>,
-    graph: map<BT.G.Reference, seq<BT.G.Reference>,
+    t: HashMap,
+    locs: map<BT.G.Reference, BC.Location>,
+    graph: map<BT.G.Reference, seq<BT.G.Reference>>
+  )
 
     // This contains reference with the empty predecessor set.
     // We use a LRU queue not because we care about the LRU,
     // but just because it happens to be a queue data structure lying around.
-    garbageQueue: LruModel.LruQueue,
-    refcounts: map<BT.G.Reference, uint64>)
+    //garbageQueue: LruModel.LruQueue,
+    //refcounts: map<BT.G.Reference, uint64>)
 
-  datatype PredecessorEdge = PredecessorEdge(src: BT.G.Reference, idx: int)
+  function Locs(t: HashMap) : map<BT.G.Reference, BC.Location>
+  {
+    map ref | ref in t.contents && t.contents[ref].loc.Some? :: t.contents[ref].loc.value
+  }
+
+  function Graph(t: HashMap) : map<BT.G.Reference, seq<BT.G.Reference>>
+  {
+    map ref | ref in t.contents :: t.contents[ref].succs
+  }
+
+  /*datatype PredecessorEdge = PredecessorEdge(src: BT.G.Reference, idx: int)
 
   function PredecessorSet(graph: map<BT.G.Reference, seq<BT.G.Reference>>, dest: BT.G.Reference) : set<PredecessorEdge>
   {
@@ -28,51 +54,68 @@ module IndirectionTableModel {
     map ref | ref in graph :: |PredecessorSet(graph, ref)|
   }
 
-  predicate Refcount0(table: IndirectionTable, ref: BT.G.Reference)
+  predicate Refcount0(self: IndirectionTable, ref: BT.G.Reference)
   {
     && ref in refcounts
     && refcounts[ref] == 0
   }
+  */
 
-  protected predicate Inv(table: IndirectionTable)
+  protected predicate Inv(self: IndirectionTable)
   {
-    && (forall ref | ref in LruModel.I(table.garbageQueue) :: Refcount0(table, ref))
-    && (forall ref | Refcount0(table, ref) :: ref in LruModel.I(table.garbageQueue))
-    && table.refcounts == GraphRefcounts(table.graph)
+    //&& (forall ref | ref in LruModel.I(self.garbageQueue) :: Refcount0(self, ref))
+    //&& (forall ref | Refcount0(self, ref) :: ref in LruModel.I(self.garbageQueue))
+    //&& self.refcounts == GraphRefcounts(self.graph)
+    && MutableMapModel.Inv(self.t)
+    && self.locs == Locs(self.t)
+    && self.graph == Graph(self.t)
   }
 
-  function RemoveLoc(table: IndirectionTable, ref: BT.G.Reference)
+  function {:opaque} RemoveLocIfPresent(self: IndirectionTable, ref: BT.G.Reference) : (self' : IndirectionTable)
+  requires Inv(self)
+  ensures Inv(self')
+  ensures self'.locs == MapRemove1(self.locs, ref)
+  ensures self'.graph == self.graph
   {
-    IndirectionTable(
-      MapRemove1(table.locs, ref),
-      table.graph,
-      table.garbageQueue,
-      table.refcounts)
+    assume self.t.count as nat < 0x10000000000000000 / 8;
+    var oldEntry := MutableMapModel.Get(self.t, ref);
+    var t := (if oldEntry.Some? then
+      MutableMapModel.Insert(self.t, ref, Entry(None, oldEntry.value.succs))
+    else
+      self.t);
+    IndirectionTable(t, Locs(t), Graph(t))
   }
 
-  function AddLoc(table: IndirectionTable, ref: BT.G.Reference, loc: LBAType.Location)
+  function {:opaque} AddLocIfPresent(self: IndirectionTable, ref: BT.G.Reference, loc: BC.Location) : (self' : IndirectionTable)
+  requires Inv(self)
+  ensures Inv(self')
+  ensures self'.graph == self.graph
+  ensures ref in self.graph ==> self'.locs == self.locs[ref := loc]
+  ensures ref !in self.graph ==> self'.locs == self.locs
   {
-    IndirectionTable(
-      table.locs[ref := loc],
-      table.graph,
-      table.garbageQueue,
-      table.refcounts)
+    assume self.t.count as nat < 0x10000000000000000 / 8;
+    var oldEntry := MutableMapModel.Get(self.t, ref);
+    var t := (if oldEntry.Some? then
+      MutableMapModel.Insert(self.t, ref, Entry(Some(loc), oldEntry.value.succs))
+    else
+      self.t);
+    IndirectionTable(t, Locs(t), Graph(t))
   }
 
-  function updateRefcountsInc(garbageQueue: LruModel.LruQueue, refcounts: map<BT.G.Reference, uint64>, oldChildren: seq<BT.G.Reference, uint64>, newChildren: seq<BT.G.Reference>, idx: uint64)
+  /*function updateRefcountsInc(garbageQueue: LruModel.LruQueue, refcounts: map<BT.G.Reference, uint64>, oldChildren: seq<BT.G.Reference, uint64>, newChildren: seq<BT.G.Reference>, idx: uint64)
   requires 0 <= idx <= |newChildren|
   {
     if idx ==
-  }
+  }*/
 
-  function UpdateAndRemoveLoc(table: IndirectionTable, ref: BT.G.Reference, children: seq<BT.G.Reference>)
+  function {:opaque} UpdateAndRemoveLoc(self: IndirectionTable, ref: BT.G.Reference, succs: seq<BT.G.Reference>) : (self' : IndirectionTable)
+  requires Inv(self)
+  ensures Inv(self')
+  ensures self'.locs == MapRemove1(self.locs, ref)
+  ensures self'.graph == self.graph[ref := succs]
   {
-    var (gq, rc) := updateRefcountsInc(table.garbageQueue, table.refcounts,
-        table.locs[ref], children, 0);
-    IndirectionTable(
-      MapRemove1(table.locs, ref),
-      table.locs[ref := children],
-      gq,
-      rc)
+    assume self.t.count as nat < 0x10000000000000000 / 8;
+    var t := MutableMapModel.Insert(self.t, ref, Entry(None, succs));
+    IndirectionTable(t, Locs(t), Graph(t))
   }
 }
